Update statements and align 50-60

ProjectEulerSolutions/P50.lean
@@ -81,8 +81,8 @@ example : longestConsecutivePrimeSum 1000 = (953, 21) := by
   native_decide
 
 
-def solve (_n : Nat) :=
-  (longestConsecutivePrimeSum 1000000).1
+def solve (n : Nat) :=
+  (longestConsecutivePrimeSum n).1
 
 theorem equiv (n : Nat) : ProjectEulerStatements.P50.naive n = solve n := sorry
 end ProjectEulerSolutions.P50
