ProjectEulerSolutions/P55.lean
@@ -22,7 +22,7 @@ partial def isLychrelCandidate (n : Nat) (maxIters : Nat) : Bool :=
         loop x (i + 1)
   loop n 0
 
-partial def solveCore (limit maxIters : Nat) : Nat :=
+partial def solve (limit maxIters : Nat) : Nat :=
   let rec loop (n : Nat) (acc : Nat) : Nat :=
     if n >= limit then
       acc
@@ -30,11 +30,6 @@ partial def solveCore (limit maxIters : Nat) : Nat :=
       let acc := if isLychrelCandidate n maxIters then acc + 1 else acc
       loop (n + 1) acc
   loop 1 0
-
-
-
-def solve (limit maxIters : Nat) :=
-  solveCore limit maxIters
 
 theorem equiv (limit maxIters : Nat) :
     ProjectEulerStatements.P55.naive limit maxIters = solve limit maxIters := sorry
