solvers/53.lean
@@ -3,4 +3,4 @@ import ProjectEulerSolutions.P53
 open ProjectEulerSolutions.P53
 
 def main : IO Unit := do
-  IO.println (solve 100 1000000)
+  IO.println solve
